\documentclass{article}
\usepackage{amsmath}
\usepackage{amssymb}
\begin{document}

\title{ML2 - 01 - LLE}
\author{Jan Laermann, Martin Nowak}
\maketitle

\section{Exercice 1: Symmetries}

Show that the minima of the cost function

\begin{equation*}
  \varepsilon(W) \sum_i |\vec{x_i} - \sum_j W_{ij} \vec{x_j}|^2
\end{equation*}

is independent to scaling, translation, and rotation.

\subsection{Scaling ($\alpha\vec{x_i}$)}

  \begin{eqnarray*}
    \varepsilon(W) &=& \sum_i |\alpha \vec{x_i} - \sum_j W_{ij} \alpha \vec{x_j}|^2\\
    &=& \sum_i |\alpha (\vec{x_i} - \sum_j W_{ij} \vec{x_j})|^2\\
    &=& \alpha^2 \sum_i |\vec{x_i} - \sum_j W_{ij} \vec{x_j}|^2
  \end{eqnarray*}

  \begin{equation*}
    \min_{\vec{W}} \varepsilon(W) = \min_{\vec{W}} \alpha^2 \varepsilon(W)
  \end{equation*}

\subsection{Translation ($\vec{x_i} + \vec{v}$)}

  \begin{eqnarray*}
    \varepsilon(W) &=& \sum_i |\vec{x_i} + \vec{v} - \sum_j W_{ij} \vec{x_j} + \vec{v}|^2\\
    &=& \sum_i |\vec{x_i} - \sum_j W_{ij} \vec{x_j} + \vec{v} - \sum_j W_{ij} \vec{v}|^2 \Big\vert \text{with } \sum_j W_{ij} = 1 \\
    &=& \sum_i |\vec{x_i} - \sum_j W_{ij} \vec{x_j}|^2\\
  \end{eqnarray*}

\subsection{Rotation ($U\vec{x_i}$)}

  \begin{eqnarray*}
    \varepsilon(W) &=& \sum_i |U \vec{x_i} - \sum_j W_{ij} U \vec{x_j}|^2\\
    &=& \sum_i |U(\vec{x_i} - \sum_j W_{ij} \vec{x_j})|^2 \Big\vert \text{with } |U\vec{v}|^2 = |\vec{v}|^2 \text{b/c U is normalized}\\
    &=& \sum_i |\vec{x_i} - \sum_j W_{ij} \vec{x_j}|^2\\
  \end{eqnarray*}

\subsection{Rotation around arbitrary point}

A rotation around an arbitrary point is a series of translation,
rotation, and translation, thus already proved above.

\section{Exercice 2: Lagrange Multipliers}

\subsection{Optimal weights for one point ($\min_{\vec{w}} \vec{w}^TC\vec{w}$)}

  \begin{eqnarray*}
    |\vec{x} - \sum_j \vec{w}_j \vec{\eta_j}|^2 &=& |\sum_j \vec{w}_j (\vec{x} - \vec{\eta_j})|^2\\
    &=& (\sum_j \vec{w}_j (\vec{x} - \vec{\eta_j}))^T (\sum_k \vec{w}_k (\vec{x} - \vec{\eta_k}))\\
    &=& \sum_{jk} \vec{w}_j \vec{w}_k (\vec{x} - \eta_j)^T(\vec{x} - \eta_k)\\
    &=& \sum_{jk} \vec{w}_j \vec{w}_k C_{jk}\\
    &=& \vec{w}^T C \vec{w}\\
  \end{eqnarray*}

\subsection{Closed solution for optimum}

  \begin{eqnarray*}
    \Lambda(\vec{w},\lambda) &=& \vec{w}^TC\vec{w} + \lambda(\vec{w}^T \vec{1} - 1)
  \end{eqnarray*}

  \begin{eqnarray*}
    \frac{\nabla\Lambda(\vec{w},\lambda)}{\delta\vec{w}} &=& 2 C \vec{w} + \lambda \vec{1} = 0\\
    \vec{w} &=& - \frac{\lambda}{2} C^{-1} \vec{1}\\
    \frac{\nabla\Lambda(\vec{w},\lambda)}{\delta\lambda} &=& \vec{w}^T \vec{1} - 1 = 0\\
    \text{substituting } \vec{w}&&\\
    (- \frac{\lambda}{2} C^{-1} \vec{1})^T \vec{1} &=& 1\\
    (C^{-1} \vec{1})^T \vec{1} &=& - \frac{2}{\lambda}\\
    \vec{1}^T C^{-1^T} \vec{1} &=& - \frac{2}{\lambda} \Big\vert \text{with } C^{-1^T} = C^{-1} \text{(C is symmetric)}\\
    \lambda &=& -\frac{2}{\vec{1}^T C^{-1} \vec{1}}\\
    \text{plugged into above eq. }&&\\
    \vec{w} &=& \frac{C^{-1} \vec{1}}{\vec{1}^T C^{-1} \vec{1}}
  \end{eqnarray*}

\subsection{Alternative calculation of closed solution}

  \begin{eqnarray*}
    C \vec{w} &=& \vec{1}\\
    \vec{w} &=& C^{-1} \vec{1}\\
    \text{scaling } k \vec{w}&&\\
    k \vec{w}^T \vec{1} &=& 1\\
    k (C^{-1} \vec{1})^T \vec{1} &=& 1\\
    k &=& \frac{1}{\vec{1}^T C^{-1^T} \vec{1}}\\
    k \vec{w} &=& \frac{C^{-1} \vec{1}}{\vec{1}^T C^{-1^T} \vec{1}}
  \end{eqnarray*}

\end{document}
